src/Ex/Mesi/MesiInv.v
@@ -247,6 +247,18 @@ Ltac solve_RsDown_by_rsDown oidx :=
 Ltac solve_NoRsI_by_rsDown oidx :=
   disc_MsgConflictsInv oidx; solve_RsDown_by_rsDown oidx.
 
+Ltac derive_NoRsI_by_no_uplock oidx msgs :=
+  assert (NoRsI oidx msgs)
+  by (solve_NoRsI_base; solve_NoRsI_by_no_uplock oidx).
+
+Ltac derive_NoRsI_by_rsDown oidx msgs :=
+  assert (NoRsI oidx msgs)
+  by (solve_NoRsI_base; solve_NoRsI_by_rsDown oidx).
+
+Ltac derive_NoRsI_by_rqDown oidx msgs :=
+  assert (NoRsI oidx msgs)
+  by (solve_NoRsI_base; solve_NoRsI_by_rqDown oidx).
+
 Ltac solve_NoRqI_base :=
   red; solve_MsgsNotExist_base.
 
